src/paths-new/Substitution.v
@@ -13,20 +13,22 @@ Require Import Weakening.
 (** * Definitions *)
 
 (** Substitution on variables: [a[u/z]] (substituting [z] with [u] in [a]). *)
+
+Definition subst_var (z: var) (u: var) (x: var): var :=
+  If x = z then u else x.
+
+Hint Unfold subst_var.
+
 Definition subst_avar (z: var) (u: var) (a: avar) : avar :=
   match a with
   | avar_b i => avar_b i
-  | avar_f x => (avar_f (If x = z then u else x))
+  | avar_f x => avar_f (subst_var z u x)
   end.
 
 Fixpoint subst_path (z: var) (u: var) (p: path) : path :=
   match p with
-  | p_var x   => p_var (subst_avar z u x)
-  | p_sel p a => p_sel (subst_path z u p) a
+  | p_sel x bs => p_sel (subst_avar z u x) bs
   end.
-
-Definition subst_paths (z: var) (u: var) (P: paths): paths :=
-  List.map (subst_path z u) P.
 
 (** Substitution on types and declarations: [T[u/z]] and [D[u/z]]. *)
 Fixpoint subst_typ (z: var) (u: var) (T: typ) { struct T } : typ :=
@@ -84,19 +86,25 @@ Definition subst_ctx (z: var) (u: var) (G: ctx) : ctx :=
 Lemma subst_fresh_avar: forall x y,
   (forall a: avar, x \notin fv_avar a -> subst_avar x y a = a).
 Proof.
-  intros. destruct* a. simpl. case_var*. simpls. notin_false.
+  intros. destruct* a. simpl. autounfold. case_var*. simpls. notin_false.
+Qed.
+
+Lemma subst_fresh_path : forall x y p,
+    x \notin fv_path p ->
+    subst_path x y p = p.
+Proof.
+  intros. destruct p. simpl. f_equal. apply* subst_fresh_avar.
 Qed.
 
 (** - in types, declarations, paths *)
-Lemma subst_fresh_typ_dec_path: forall x y,
+Lemma subst_fresh_typ_dec: forall x y,
   (forall T : typ  , x \notin fv_typ  T  -> subst_typ  x y T  = T ) /\
-  (forall D : dec  , x \notin fv_dec  D  -> subst_dec  x y D  = D ) /\
-  (forall P : path , x \notin fv_path P  -> subst_path x y P  = P ).
+  (forall D : dec  , x \notin fv_dec  D  -> subst_dec  x y D  = D ).
 Proof.
-  intros x y. apply typ_mutind; intros; simpls; f_equal*. apply subst_fresh_avar. assumption.
+  intros x y. apply typ_mutind; intros; simpls; f_equal*. apply* subst_fresh_path.
 Qed.
 
-Definition subst_fresh_typ(x y: var) := proj1 (subst_fresh_typ_dec_path x y).
+Definition subst_fresh_typ(x y: var) := proj1 (subst_fresh_typ_dec x y).
 
 (** - in terms, values, and definitions *)
 Lemma subst_fresh_trm_val_def_defs: forall x y,
@@ -106,7 +114,7 @@ Lemma subst_fresh_trm_val_def_defs: forall x y,
   (forall ds: defs, x \notin fv_defs ds -> subst_defs x y ds = ds).
 Proof.
   intros x y. apply trm_mutind; intros; simpls; f_equal*;
-    (apply* subst_fresh_avar || apply* subst_fresh_typ_dec_path).
+    (apply* subst_fresh_typ_dec || apply* subst_fresh_path).
 Qed.
 
 Lemma fv_ctx_types_push_eq : forall G x T,
@@ -175,7 +183,7 @@ Proof.
     apply invert_fv_ctx_types_push in N. destruct N as [N1 N2].
     unfold subst_ctx in *. rewrite map_push.
     rewrite (IH N2).
-    rewrite ((proj1 (subst_fresh_typ_dec_path _ _)) _ N1).
+    rewrite ((proj1 (subst_fresh_typ_dec _ _)) _ N1).
     reflexivity.
 Qed.
 
@@ -193,57 +201,63 @@ Lemma subst_open_commut: forall x y u a n,
     subst_avar x y (open_rec_avar n u a)
     = open_rec_avar n (subst_fvar x y u) (subst_avar x y a).
 Proof.
-  intros. unfold subst_fvar, subst_avar, open_avar, open_rec_avar. destruct a.
+  intros. unfold subst_fvar, subst_avar, open_avar, open_rec_avar. destruct a; autounfold.
   + repeat case_if; auto.
   + case_var*.
 Qed.
 
+(** - paths *)
+Lemma subst_open_commut_path: forall p n x y u,
+     subst_path x y (open_rec_path n u p)
+     = open_rec_path n (subst_fvar x y u) (subst_path x y p).
+Proof.
+  Admitted.
+
 (** - types and declarations *)
-Lemma subst_open_commute_typ_dec: forall x y u,
+Lemma subst_open_commut_typ_dec: forall x y u,
   (forall t : typ, forall n: nat,
      subst_typ x y (open_rec_typ n u t)
      = open_rec_typ n (subst_fvar x y u) (subst_typ x y t)) /\
   (forall D : dec, forall n: nat,
      subst_dec x y (open_rec_dec n u D)
-     = open_rec_dec n (subst_fvar x y u) (subst_dec x y D)) /\
-  (forall p : path, forall n: nat,
-     subst_path x y (open_rec_path n u p)
-     = open_rec_path n (subst_fvar x y u) (subst_path x y p)).
+     = open_rec_dec n (subst_fvar x y u) (subst_dec x y D)).
 Proof.
-  intros. apply typ_mutind; intros; simpl; f_equal*.
-  destruct a; simpl. case_if*. case_var*.
+  intros. apply typ_mutind; intros; simpl; f_equal*. apply subst_open_commut_path.
 Qed.
 
-Lemma subst_open_commute_typ_dec_p: forall x y u,
+Lemma subst_open_commut_path_p: forall p n x y u,
+    subst_path x y (open_rec_path_p n u p)
+    = open_rec_path_p n (subst_path x y u) (subst_path x y p).
+Proof.
+  intros. Admitted.
+
+Lemma subst_open_commut_typ_dec_p: forall x y u,
   (forall t : typ, forall n: nat,
      subst_typ x y (open_rec_typ_p n u t)
      = open_rec_typ_p n (subst_path x y u) (subst_typ x y t)) /\
   (forall D : dec, forall n: nat,
      subst_dec x y (open_rec_dec_p n u D)
-     = open_rec_dec_p n (subst_path x y u) (subst_dec x y D)) /\
-  (forall p : path, forall n: nat,
-     subst_path x y (open_rec_path_p n u p)
-     = open_rec_path_p n (subst_path x y u) (subst_path x y p)).
+     = open_rec_dec_p n (subst_path x y u) (subst_dec x y D)).
 Proof.
   intros. apply typ_mutind; intros; simpl; f_equal*.
-  destruct a; simpl. case_if*. case_var*.
+  apply subst_open_commut_path_p.
 Qed.
 
 (** - types only *)
 Lemma subst_open_commut_typ: forall x y u T,
   subst_typ x y (open_typ u T) = open_typ (subst_fvar x y u) (subst_typ x y T).
 Proof.
-  intros. apply* subst_open_commute_typ_dec.
+  intros. apply subst_open_commut_typ_dec.
 Qed.
 
 Lemma subst_open_commut_typ_p: forall x y u T,
   subst_typ x y (open_typ_p u T) = open_typ_p (subst_path x y u) (subst_typ x y T).
 Proof.
-  intros. apply* subst_open_commute_typ_dec_p.
+  intros. apply* subst_open_commut_typ_dec_p.
 Qed.
 
 (** - terms, values, definitions, and list of definitions *)
-Lemma subst_open_commute_trm_val_def_defs: forall x y u,
+Lemma subst_open_commut_trm_val_def_defs: forall x y u,
   (forall t : trm, forall n: nat,
      subst_trm x y (open_rec_trm n u t)
      = open_rec_trm n (subst_fvar x y u) (subst_trm x y t)) /\
@@ -258,10 +272,10 @@ Lemma subst_open_commute_trm_val_def_defs: forall x y u,
      = open_rec_defs n (subst_fvar x y u) (subst_defs x y ds)).
 Proof.
   intros. apply trm_mutind; intros; simpl; f_equal*;
-  apply* subst_open_commute_typ_dec.
+  apply subst_open_commut_path || apply subst_open_commut_typ_dec.
 Qed.
 
-Lemma subst_open_commute_trm_val_def_defs_p: forall x y u,
+Lemma subst_open_commut_trm_val_def_defs_p: forall x y u,
   (forall t : trm, forall n: nat,
      subst_trm x y (open_rec_trm_p n u t)
      = open_rec_trm_p n (subst_path x y u) (subst_trm x y t)) /\
@@ -276,7 +290,7 @@ Lemma subst_open_commute_trm_val_def_defs_p: forall x y u,
      = open_rec_defs_p n (subst_path x y u) (subst_defs x y ds)).
 Proof.
   intros. apply trm_mutind; intros; simpl; f_equal*;
-  apply* subst_open_commute_typ_dec_p.
+  apply subst_open_commut_typ_dec_p || apply subst_open_commut_path_p.
 Qed.
 
 (** - terms only *)
@@ -284,14 +298,14 @@ Lemma subst_open_commut_trm: forall x y u t,
     subst_trm x y (open_trm u t)
     = open_trm (subst_fvar x y u) (subst_trm x y t).
 Proof.
-  intros. apply* subst_open_commute_trm_val_def_defs.
+  intros. apply* subst_open_commut_trm_val_def_defs.
 Qed.
 
 Lemma subst_open_commut_trm_p: forall x y u t,
     subst_trm x y (open_trm_p u t)
     = open_trm_p (subst_path x y u) (subst_trm x y t).
 Proof.
-  intros. apply* subst_open_commute_trm_val_def_defs_p.
+  intros. apply* subst_open_commut_trm_val_def_defs_p.
 Qed.
 
 (** - definitions only *)
@@ -299,14 +313,14 @@ Lemma subst_open_commut_defs: forall x y u ds,
     subst_defs x y (open_defs u ds)
     = open_defs (subst_fvar x y u) (subst_defs x y ds).
 Proof.
-  intros. apply* subst_open_commute_trm_val_def_defs.
+  intros. apply* subst_open_commut_trm_val_def_defs.
 Qed.
 
 Lemma subst_open_commut_defs_p: forall x y u ds,
     subst_defs x y (open_defs_p u ds)
     = open_defs_p (subst_path x y u) (subst_defs x y ds).
 Proof.
-  intros. apply* subst_open_commute_trm_val_def_defs_p.
+  intros. apply* subst_open_commut_trm_val_def_defs_p.
 Qed.
 
 (** The following lemmas state that opening a symbol with a variable [y]
@@ -338,7 +352,7 @@ Lemma subst_intro_typ: forall x u T, x \notin (fv_typ T) ->
   open_typ u T = subst_typ x u (open_typ x T).
 Proof.
   introv Fr. unfold open_typ. rewrite* subst_open_commut_typ.
-  destruct (@subst_fresh_typ_dec_path x u) as [Q _]. rewrite* (Q T).
+  destruct (@subst_fresh_typ_dec x u) as [Q _]. rewrite* (Q T).
   unfold subst_fvar. case_var*.
 Qed.
 
@@ -378,7 +392,7 @@ Proof.
     simpl in Eq. case_if~.
 Qed.
 
-Ltac subst_solver :=
+Ltac subst_fresh_solver :=
   fresh_constructor;
   subst_open_fresh;
   match goal with
@@ -388,7 +402,7 @@ Ltac subst_solver :=
         by (unfold subst_ctx; rewrite map_concat, map_single; reflexivity);
     rewrite <- concat_assoc; rewrite B;
     try match goal with
-            | [ |- _; _; _ ⊢ _ _ _ :: _ ] =>
+            | [ |- _; _; _; _ ⊢ _ _ _ :: _ ] =>
               assert (z = subst_fvar x y z) as Hxyz by (unfold subst_fvar; rewrite~ If_r);
                 rewrite Hxyz at 1
             end;
@@ -397,6 +411,17 @@ Ltac subst_solver :=
     rewrite <- B,concat_assoc; unfold subst_ctx;
     auto using weaken_ty_trm, ok_push, ok_concat_map
   end.
+
+Ltac subst_tydef_solver :=
+  match goal with
+    | [ H: forall G3 G4 x, _,
+          Hok: ok _,
+          Hx: ?x \notin fv_ctx_types _,
+          Hy: _ & _ ⊢ _ : _ |- _] =>
+      specialize (H _ _ _ eq_refl Hok Hx);
+      try solve [rewrite subst_open_commut_defs_p in H;
+                 rewrite subst_open_commut_typ_p in H; eauto]
+    end.
 
 (** * Substitution Lemma *)
 (** [G1, x: S, G2 ⊢ t: T]            #<br>#
@@ -441,18 +466,22 @@ Lemma subst_rules: forall y S,
     x \notin fv_ctx_types G1 ->
     G1 & (subst_ctx x y G2) ⊢ tvar y : subst_typ x y S ->
     G1 & (subst_ctx x y G2) ⊢ subst_trm x y t : subst_typ x y T) /\
-  (forall p P G d D, p; P; G ⊢ d : D -> forall G1 G2 x,
+  (forall z bs P G d D, z; bs; P; G ⊢ d : D -> forall G1 G2 x,
     G = G1 & x ~ S & G2 ->
     ok (G1 & x ~ S & G2) ->
     x \notin fv_ctx_types G1 ->
+    x <> z ->
+    y <> z ->
     G1 & (subst_ctx x y G2) ⊢ tvar y : subst_typ x y S ->
-    subst_path x y p; subst_paths x y P; G1 & (subst_ctx x y G2) ⊢ subst_def x y d : subst_dec x y D) /\
-  (forall p P G ds T, p; P; G ⊢ ds :: T -> forall G1 G2 x,
+    subst_var x y z; bs; P; G1 & (subst_ctx x y G2) ⊢ subst_def x y d : subst_dec x y D) /\
+  (forall z bs P G ds T, z; bs; P; G ⊢ ds :: T -> forall G1 G2 x,
     G = G1 & x ~ S & G2 ->
     ok (G1 & x ~ S & G2) ->
     x \notin fv_ctx_types G1 ->
+    x <> z ->
+    y <> z ->
     G1 & (subst_ctx x y G2) ⊢ tvar y : subst_typ x y S ->
-    subst_path x y p; subst_paths x y P; G1 & (subst_ctx x y G2) ⊢ subst_defs x y ds :: subst_typ x y T) /\
+    subst_var x y z; bs; P; G1 & (subst_ctx x y G2) ⊢ subst_defs x y ds :: subst_typ x y T) /\
   (forall G T U, G ⊢ T <: U -> forall G1 G2 x,
     G = G1 & x ~ S & G2 ->
     ok (G1 & x ~ S & G2) ->
@@ -461,8 +490,8 @@ Lemma subst_rules: forall y S,
     G1 & (subst_ctx x y G2) ⊢ subst_typ x y T <: subst_typ x y U).
 Proof.
   introv. apply rules_mutind; intros; subst; simpl;
-            try (subst_solver || rewrite subst_open_commut_typ_p);
-            simpl in *; eauto 4.
+            try (subst_fresh_solver || rewrite subst_open_commut_typ_p);
+            simpl in *; autounfold; eauto 4.
   - Case "ty_var".
     cases_if.
     + apply binds_middle_eq_inv in b; subst; assumption.
@@ -471,17 +500,16 @@ Proof.
       constructor. rewrite <- H1.
       unfold subst_ctx. rewrite <- map_concat.
       apply binds_map; auto. apply ok_concat_map. apply* ok_remove.
+  - Case "ty_new_elim".
+    asserts_rewrite (subst_path x y p • a = (subst_path x y p) • a).
+    destruct p. reflexivity. eauto.
   - Case "ty_rec_intro".
     constructor. rewrite <- subst_open_commut_typ_p. simpl in *. auto.
-  - Case "ty_defs_new".
-    constructor.
-    specialize (H _ _ _ eq_refl H1 H2 H3).
-    rewrite subst_open_commut_defs_p in H.
-    rewrite subst_open_commut_typ_p in H. simpl in *. apply* H.
+  - Case "ty_def_new".
+    subst_tydef_solver.
   - Case "ty_def_path".
-    constructor.
-    specialize (H _ _ _ eq_refl H1 H2 H3). apply* H. intro.
-
+    subst_tydef_solver.
+    apply* ty_def_path. intro. case_if; case_if; subst; eauto.
   - Case "ty_defs_cons".
     constructor*.
     rewrite <- subst_label_of_def.
@@ -491,10 +519,10 @@ Qed.
 (** The substitution lemma for term typing.
     This lemma corresponds to Lemma 3.14 in the paper. *)
 Lemma subst_ty_trm: forall y S G x t T,
-    G & x ~ S ⊢ t : T ->(
+    G & x ~ S ⊢ t : T ->
     ok (G & x ~ S) ->
     x \notin fv_ctx_types G ->
-    G ⊢ trm_var (avar_f y) : subst_typ x y S ->
+    G ⊢ tvar y : subst_typ x y S ->
     G ⊢ subst_trm x y t : subst_typ x y T.
 Proof.
   intros.
@@ -507,13 +535,14 @@ Proof.
   unfold subst_ctx. rewrite map_empty, concat_empty_r. assumption.
 Qed.
 
+(*
 (** The substitution lemma for definition typing. *)
-Lemma subst_ty_defs: forall y S G x ds T,
-    G & x ~ S ⊢ ds :: T ->
+Lemma subst_ty_defs: forall y S G x ds T z bs P,
+    z; bs; P; G & x ~ S ⊢ ds :: T ->
     ok (G & x ~ S) ->
     x \notin fv_ctx_types G ->
     G ⊢ trm_var (avar_f y) : subst_typ x y S ->
-    G ⊢ subst_defs x y ds :: subst_typ x y T.
+    z; bs; P G ⊢ subst_defs x y ds :: subst_typ x y T.
 Proof.
   intros.
   apply (proj53 (subst_rules y S)) with (G1:=G) (G2:=empty) (x:=x) in H;
@@ -521,4 +550,4 @@ Proof.
   - unfold subst_ctx in H. rewrite map_empty, concat_empty_r in H.
     auto.
   - unfold subst_ctx. rewrite map_empty. rewrite concat_empty_r. assumption.
-Qed.
+Qed.*)
